lecture11/intlist-bound.dfy
@@ -16,51 +16,48 @@ requires 0 < length(l)
   case Cons(j,js) => max(j,maxList(js))
 }
 
-
-
-lemma maxList_exceeds(l : list<int>)
-requires 0 < length(l)
-ensures exceeds(maxList(l) + 1,l)
-{
-  match l case Nil => {}
-  case Cons(j,Nil) => {}
-  case Cons(j,js) => {
-    assert(maxList(l) == max(j,maxList(js)));
-    assert exceeds(maxList(js)+1, js);
-    assert maxList(l) +1 > j;
-    /* maxList(js) + 1 >> js
-       maxList(l) == max(j,maxList(js))
-       maxList(l) + 1 > j && maxList(l) + 1 > maxList(js)
-       */
-    assert maxList(l) + 1>= maxList(js) +1;
-    // and also maxList(js) + 1 >> js
-    exceeds_ge(maxList(l) + 1, maxList(js) + 1, js);
-    assert exceeds(maxList(l) + 1 , js);
-    // maxList(l) + 1 >> js
-  }
-}
-
-// i >= j && j >= k ==> i>= k
-
 lemma exceeds_ge(i:int, j :int, l : list<int>)
 requires i >= j requires exceeds(j,l) // j >> l
 ensures exceeds(i,l) // i >> l
 {}
 
+lemma maxList_exceeds(l : list<int>)
+requires 0 < length(l)
+ensures exceeds(maxList(l) + 1,l)
+{ 
+ match l
+ case Nil => {}
+ case Cons(j,Nil) => {}
+ case Cons(j,js) => {
+  //maxList(l) + 1 >j && exceeds(maxList(js)+1,js);
+  //max(j,maxList(js))+1 > j
+  assert maxList(l) == max(j,maxList(js));
+  assert maxList(l) + 1 > j;
+  assert exceeds(maxList(js)+1,js);
+  exceeds_ge(maxList(l)+1,maxList(js)+1,js);
+  assert exceeds(maxList(l)+1,js);
+ }
+}
+
+// i >= j && j >= k ==> i>= k
+ 
+
+
 lemma boundExists(l : list<int>)
   ensures exists m :: exceeds(m,l)
   {
     match l
-    case Nil => {assert exceeds(-3,l);}
+    case Nil => {assert exceeds(-7,l);}
     case Cons(j,Nil) => {assert exceeds(j+1,l);}
     case Cons(j,js) => {
       boundExists(js);
-      var m0 :| exceeds(m0,js);
-      assert max(m0,j) +1 >j;
-      assert max(m0,j) + 1 > m0;
-      exceeds_ge(max(m0,j)+1,m0,js);
-      assert exceeds(max(m0,j)+1,l);
+      var n :| exceeds(n,js);
+      assert max(n,j)+1 > n;
+      assert max(n,j)+1 > j;
+      exceeds_ge(max(n,j)+1,n,js);
+      assert exceeds(max(n,j)+1,l);
     }
-  }
+  } 
+
 
 // flip quantifiers, prove something else
